\documentclass[12pt]{extarticle}
\include{QuantumCommands}

\begin{document}
\atitle{3}                     
 
\section*{Problem 8.}
\begin{enumerate}
\item Let $\Delta x \Delta p \approx \hbar$ then \[E = \frac{\Delta p^2}{2m} - \frac{e^2}{\Delta x} = \frac{1}{\Delta x^2} \frac{\hbar^2}{2m} - \frac{e^2}{\Delta x}\]
Now, we minimize the energy with respect to $\Delta x$: 
\[E' = - \frac{2}{\Delta x^3} \frac{\hbar^2}{2m} + \frac{e^2}{\Delta x^2} = 0 \quad \text{gives} \quad \Delta x = \frac{\hbar^2}{me^2}\]
Now plugging in, \[E = \frac{m^2 e^4}{\hbar^4} \frac{\hbar^2}{2m} - \frac{m e^4}{\hbar^2} = - \frac{m e^4}{2 \hbar^2}\] 

\item $\Delta E \Delta t \approx \hbar$. Assuming that $\Delta t \approx \tau_{1/2} = 4 \times 10^{-6} \mathrm{s}$ then $\Delta E \approx 2.6 \times 10^{-29} \mathrm{J} = 1.6 \times 10^{-10} \mathrm{eV}$.

\item Model a ballanced pencil as an inverted physical pendulum with equation of motion \[\ddot{\theta} = \frac{g}{\ell_{CM}} \frac{m \ell^2}{m \ell^2 + I_{CM}} \sin{\theta}\]
where $l_{CM}$ is the height of the center of mass, $m$ is the mass, and $I_{CM}$ is the moment of inertia about the center of mass. Define $\omega_0 =  \sqrt{\frac{g}{\ell_{CM}} \frac{m \ell^2}{m \ell^2 + I_{CM}}}$. Now, applying a small angle approximation, the general solution is given by: \[\theta(t) = \theta_0 \cosh{\omega t} + \frac{\dot{\theta}_0}{\omega_0} \sinh{\omega_0 t} \] 

Let $\zeta_0 = \frac{\dot{\theta}_0}{\omega_0}$ then,  \[\theta(t) = \theta_0 \cosh{\omega t} + \zeta_0 \sinh{\omega_0 t} = \frac{1}{2} (\theta_0 + \zeta_0) e^{\omega_0 t} + \frac{1}{2}(\theta_0 - \zeta_0) e^{-\omega_0 t} \] 
Since we are looking for a maximum time, we assume that the time is much larger than $\frac{1}{\omega_0}$ so that the decaying exponential term can be ignored. Then, \[\theta(t) = \frac{1}{2} (\theta_0 + \zeta_0) e^{\omega_0 t} \]
Thus, \[t = \frac{1}{\omega_0} \log{\left(\frac{2 \theta_{max}}{\theta_0 + \zeta_0} \right)}\] 
To maximize $t$, we minimize the denominator $\theta_0 + \zeta_0$. However, from the uncertianty principle, when we try to set $\theta = 0$ the uncertainty in coordinates effectivly puts the true initial conditions at $\theta_0 = \frac{\Delta x}{\ell_{CM}}$ and $\dot{\theta}_0 = \frac{\Delta p}{m \ell}$ so $\theta_0 \dot{\theta}_0 \approx \frac{\hbar}{m \ell^2}$ i.e. $\theta_0 \zeta_0 \approx \frac{\hbar}{m \ell^2 \omega_0}$.

Now set $\deriv{t}{\theta_0} = 0$ which is equivalent to $\deriv{}{\theta_0} (\theta_0 + \zeta_0) = 0$ so $1 - \frac{1}{\theta_0^2}\frac{\hbar}{m \ell^2 \omega_0} = 0$ so the maximum time occurs for \[\theta_0 = \sqrt{\frac{\hbar}{m \ell^2 \omega_0}} \text{  giving  } \zeta_0 = \sqrt{\frac{\hbar}{m \ell^2 \omega_0}} \]
which corresponds to a time, \[t = \frac{1}{\omega_0} \log{\left(\theta_{max} \sqrt{\frac{m \ell^2 \omega_0}{\hbar}} \right)} \] 
For $\ell_{CM} = 6 \mathrm{cm}$, $m = 10 \mathrm{g}$, $I_{CM} = \frac{1}{3} m \ell^3$, and $\theta_{max} = 15^\circ$, then the maximum ballance time occurs for $\theta_0 = 1.62 \times 10^{-16}$ giving $t = 3.16 \: \mathrm{s}$.

\end{enumerate}

\section*{Problem 9.}

\begin{enumerate}
\item At $t = 0$, let \[\psi_0(x) = \frac{1}{(2 \pi)^{1/4} d^{1/2}} \exp{\left[-\frac{x^2}{4 d^2} + i \frac{p_0}{\hbar} x \right]}\]
Applying the Fourier transform to the Schrodinger equation, 

\[ \mathcal{F}_x\left[ \hbar \frac{\partial}{\partial t} \psi(x, t) \right] = \mathcal{F}_x\left[ - \frac{\hbar^2}{2m} \frac{\partial^2}{\partial x^2} \psi(x,t) \right] \]
\[ \frac{\partial}{\partial t} \tilde{\psi}(k, t) = - i \frac{\hbar k^2}{2m} \tilde{\psi}(k,t) \]

Thus, \[ \tilde{\psi}(k, t) = \tilde{\psi}_0(k) \exp{\left( - i \frac{\hbar k^2}{2m} t \right)}\]


Now, 
\[\tilde{\psi_0}(k) = \frac{1}{\sqrt{2 \pi}} \frac{1}{(2 \pi)^{1/4} d^{1/2}} \int_{-\infty}^{\infty} \exp{\left[-\frac{x^2}{4 d^2} + i \frac{p_0}{\hbar} x - i k x \right]} \d{x} \]

Now expanding the exponent with $q = \frac{p_0}{\hbar}$:

\[-\frac{x^2}{4 d^2} + i q x - i k x  = -\frac{1}{4 d^2} [x + 2i d^2 (k - q)]^2 - d^2(k-q)^2 \]

Therefore, 
\begin{align*}
\tilde{\psi_0}(k) &= \frac{1}{\sqrt{2 \pi}} \frac{1}{(2 \pi)^{1/4} d^{1/2}} \int_{-\infty}^{\infty} \exp{\left[-\frac{1}{4 d^2} [x + 2i d^2 (k - q)]^2 - d^2(k-q)^2 \right] \d{x}} \\
&= \frac{1}{\sqrt{2 \pi}} \frac{1}{(2 \pi)^{1/4} d^{1/2}} \exp{\left[- d^2(k-q)^2 \right]} \int_{-\infty}^{\infty} \exp{\left[-\frac{1}{4 d^2} u^2 \right]} \d{u} \\ &= \frac{1}{\sqrt{2 \pi}} \frac{2 d \sqrt{\pi}}{(2 \pi)^{1/4} d^{1/2}} \exp{\left[- d^2(k-q)^2 \right]} = \frac{1}{(2 \pi)^{1/4} (2/d)^{1/2}} \exp{\left[- d^2(k-q)^2 \right]}
\end{align*}
So, \[ \tilde{\psi}(k, t) = \frac{(2d)^{1/2}}{(2 \pi)^{1/4}} \exp{\left[ - d^2(k-q)^2 - i \frac{\hbar k^2}{2m} t \right]}\]
Applying the inverse transform, 
\[\psi(x, t) =  \frac{1}{\sqrt{2 \pi}} \frac{(2d)^{1/2}}{(2 \pi)^{1/4}} \int_{-\infty}^{\infty} \exp{\left[ - d^2(k-q)^2 - i \frac{\hbar k^2}{2m} t + ikx \right]} \d{k}  \]
Expanding the exponent, 
\begin{align*}
- d^2(k-q)^2 &- i \frac{\hbar k^2}{2m} t + ikx = - d^2(k - q)^2 -  \frac{i \hbar t}{2m} (k - q)^2 -  \frac{i \hbar t}{m} kp +  \frac{i \hbar t}{2m} q^2 + ikx \\ & = -\left[d^2 + \frac{i \hbar t}{2m} \right] (k - q)^2 + i \left(x - \frac{p}{m} t \right) (k - q) + iqx - \frac{i \hbar t}{2m} q^2  \\ &= -\left[d^2 + \frac{i \hbar t}{2m} \right] \left[k - q - \frac{i}{2 \tilde{d}^2} \left(x - \frac{p}{m} t \right) \right]^2 - \frac{1}{4 \tilde{d}^2} \left(x - \frac{p}{m} t \right)^2 + iqx - \frac{i \hbar t}{2m} q^2
\end{align*}
with $\tilde{d}^2 = \left[d^2 + \frac{i \hbar t}{2m} \right]$ then, 

\begin{align*}
 \psi(x, t) &=  \frac{1}{\sqrt{2 \pi}} \frac{(2d)^{1/2}}{(2 \pi)^{1/4}} \int_{-\infty}^{\infty} \exp{\left[-\tilde{d}^2 u^2 - \frac{1}{4 \tilde{d}^2} \left(x - \frac{p}{m} t \right)^2 + iqx - \frac{i \hbar t}{2m} q^2 \right]} \d{u}  \\ &= \frac{1}{\tilde{d}}\frac{\sqrt{\pi}}{\sqrt{2 \pi}} \frac{(2d)^{1/2}}{(2 \pi)^{1/4}} \exp{\left[- \frac{1}{4 \tilde{d}^2} \left(x - \frac{p}{m} t \right)^2 + iqx - \frac{i \hbar t}{2m} q^2 \right]} \\ &= \frac{1}{(2 \pi)^{1/4} d^{1/2} \sqrt{1 + \frac{i \hbar t}{2md^2}}} \exp{\left[- \frac{\left(x - \frac{p}{m} t \right)^2}{4 d^2 \left(1 + \frac{i \hbar t}{2md^2} \right)} + i \frac{p_0}{\hbar}x - \frac{i p_0^2 t}{2m \hbar} \right]}
\end{align*}

\item Let $G(x - x', t) = \bra{x} e^{-i \hat{H} t /\hbar} \ket{x'}$. Then \[i \hbar \frac{\partial}{\partial t} G(x - x', t) = i \hbar \bra{x} \frac{1}{i\hbar} \hat{H} e^{-i \hat{H} t /\hbar} \ket{x'} = \bra{x} \hat{H} e^{-i \hat{H} t /\hbar} \ket{x'} \]
But, $\hat{H} = \frac{1}{2m} \hat{p}^2$ so $\bra{x} \hat{H} \ket{\psi} = -\frac{\hbar^2}{2m} \frac{\partial^2}{\partial x^2} \inner{x}{\psi}$. Thus,
\[i \hbar \frac{\partial}{\partial t} G(x - x', t) = \bra{x} \hat{H} e^{-i \hat{H} t /\hbar} \ket{x'} = -\frac{\hbar^2}{2m} \frac{\partial^2}{\partial x^2} \bra{x} e^{-i \hat{H} t /\hbar} \ket{x'} = -\frac{\hbar^2}{2m} \frac{\partial^2}{\partial x^2} G(x - x', t)  \]
Futhermore, at $t = 0$, $G(x - x', 0) = \bra{x} \mathbf{1} \ket{x'} = \inner{x}{x'} = \delta(x - x')$. 

\item \[\psi(x, t) = \inner{x}{\psi(t)} = \bra{x} e^{-i \hat{H} t /\hbar} \ket{\psi_0} = \int_{-\infty}^{\infty} \bra{x} e^{-i \hat{H} t /\hbar} \ket{x'} \! \inner{x'}{\psi_0} \d{x'} = \int_{-\infty}^{\infty} G(x - x', t) \psi_0(x') \d{x'}\]

\item Taking the Fouier Transform of, \[i \hbar \frac{\partial}{\partial t} G(x - x', t) = -\frac{\hbar^2}{2m} \frac{\partial^2}{\partial x^2} G(x - x', t)  \]
we obtain: \[i \hbar \frac{\partial}{\partial t} \tilde{G}(k, t) = \frac{\hbar^2 k^2}{2m} \tilde{G}(k, t)\]
Therefore, \[\tilde{G}(k, t) = \exp{\left(- i \frac{\hbar k^2}{2m} \right)} \tilde{G_0}(k) =  \frac{1}{\sqrt{2 \pi}} \exp{\left(- i \frac{\hbar k^2}{2m} t \right)} \]
because $G_0(x - x') = \delta(x - x')$ so $\tilde{G}(k) = \frac{1}{\sqrt{2 \pi}}$. Then applying the inverse Fourier transform, \[G(x - x', t) = \frac{1}{2 \pi} \int_{-\infty}^{\infty} e^{ik(x - x')} \exp{\left( - i \frac{\hbar k^2}{2m} t \right)} \d{k} \] 
The exponent is $-\frac{i \hbar t}{2 m} \left(k^2 - \frac{2m}{\hbar t} k (x - x') \right) = -\frac{i \hbar t}{2 m} \left(k^2 - \frac{m}{\hbar t} (x - x') \right)^2 + \frac{im}{2 \hbar t} (x - x')^2$. Thus,
\begin{align*}
G(x - x', t) &= \frac{1}{2 \pi} \int_{-\infty}^{\infty} \exp{\left[-\frac{i \hbar t}{2 m} \left(k^2 - \frac{m}{\hbar t} (x - x') \right)^2 + \frac{im}{2 \hbar t} (x - x')^2 \right]} \d{k} \\ &= \frac{1}{2 \pi} \exp{\left[\frac{im}{2 \hbar t} (x - x')^2 \right]} \int_{-\infty}^{\infty} \sqrt{\frac{2m}{i \hbar t}} \exp{\left( - u^2 \right)} \d{u}  = \sqrt{\frac{m}{ 2 \pi  i \hbar t}} \exp{\left[\frac{im}{2 \hbar t} (x - x')^2 \right]} 
\end{align*}

We verify the normalization of this Green's function by applying it to the gaussian wave packet of part $(a)$,
\begin{align*}
\psi(x, t) &= \int_{-\infty}^{\infty} G(x - x', t) \psi_0(x') \d{x'} \\ &= \int_{-\infty}^{\infty} \sqrt{\frac{m}{2 \pi i \hbar t}} \exp{\left[\frac{im}{2 \hbar t} (x - x')^2 \right]} \frac{1}{(2 \pi)^{1/4} d^{1/2}} \exp{\left[-\frac{x^2}{4 d^2} + i \frac{p_0}{\hbar} x \right]} \d{x'} \\
&= \sqrt{\frac{m}{2 \pi i \hbar t}} \frac{1}{(2 \pi)^{1/4} d^{1/2}} \int_{-\infty}^{\infty} \exp{\left[\frac{im}{2 \hbar t} (x - x')^2 -\frac{x'^2}{4 d^2} + i \frac{p_0}{\hbar} x' \right]} \d{x'} \\
&= \sqrt{\frac{m}{2 \pi i \hbar t}} \frac{1}{(2 \pi)^{1/4} d^{1/2}} \int_{-\infty}^{\infty} \exp{\left[ \left(\frac{im}{2 \hbar t} - \frac{1}{4 d^2} \right) x'^2 + \left(i \frac{p_0}{\hbar} - \frac{im}{\hbar t} x \right)x' + \frac{im}{2\hbar t} x^2 \right]} \d{x'}
\end{align*}

Let $a = \left(\frac{im}{2 \hbar t} - \frac{1}{4 d^2} \right)$, $b = \left(i \frac{p_0}{\hbar} - \frac{im}{\hbar t} x \right)$, $c = \frac{im}{2\hbar t} x^2$, and $N = \sqrt{\frac{m}{2 \pi i \hbar t}} \frac{1}{(2 \pi)^{1/4} d^{1/2}}$ \\
Then,
\begin{align*}
\psi(x, t) &= N \int_{-\infty}^{\infty} \exp{\left[ a x'^2 + bx' + c \right]} \d{x'} = N \int_{-\infty}^{\infty}  \exp{\left[a \left(x' + \frac{b}{2a} \right)^2 - \frac{b^2}{4a} + c\right]} \d{x'} \\ &= N \exp{\left[- \frac{b^2}{4a} + c\right]} \int_{-\infty}^{\infty}  \exp{\left[ a \left(x' + \frac{b}{2a} \right)^2\right]} \d{x'} = N \sqrt{\frac{\pi}{-a}} \exp{\left[- \frac{b^2}{4a} + c\right]}
\end{align*}
So pluggin in, 
\begin{align*}
\psi(x, t) &= \sqrt{\frac{m}{2 \pi i \hbar t}} \frac{\sqrt{\pi}}{(2 \pi)^{1/4} d^{1/2}} \frac{1}{\sqrt{\frac{m}{2i \hbar t} + \frac{1}{4 d^2}}} \exp{\left[\frac{\left(i \frac{p_0}{\hbar} - \frac{im}{\hbar t} x \right)^2}{4 \left(\frac{m}{2i \hbar t} + \frac{1}{4 d^2} \right)} + \frac{im}{2\hbar t} x^2 \right]} \\ &= \frac{1}{(2 \pi)^{1/4} d^{1/2} \left(1 + \frac{i \hbar t}{2md^2} \right)} \exp{\left[ - \frac{\left(x - \frac{p_0}{m} t\right)^2}{4 d^2 \left(1 + \frac{i \hbar t}{2 m d^2} \right)} + i \frac{p_0}{\hbar}x - \frac{i p_0^2 t}{2m \hbar} \right]}
\end{align*}

\end{enumerate}

\section*{Problem 10.}

Let $\hat{X} = \hat{x} - \left<x\right>$ and $\hat{P} = \hat{p} - \left< p \right>$. Take $\ket{\psi_\alpha} = (\hat{X} - i \alpha \hat{P}) \ket{\psi}$. Then expanding $\inner{\psi_\alpha}{\psi_\alpha} \ge 0$ gives the uncertainty relation. If $\psi$ saturates the uncertianty relation then the discriminant of $\inner{\psi_\alpha}{\psi_\alpha}$ is zero therefore for $\alpha = -\frac{\hbar}{2 \Delta p^2} = -\frac{\Delta x}{\Delta p} = -\frac{2\Delta x^2}{\hbar}$ the quadratic form $\inner{\phi_\alpha}{\psi_\alpha} = 0$. Thus, \\ $(\hat{X} - i \alpha \hat{P}) \ket{\psi} = 0$ so take, \[\bra{x} (\hat{X} - i \alpha \hat{P}) \ket{\psi} = (x - \left< x \right>) \psi(x) - i \alpha \left(\frac{\hbar}{i} \frac{\partial}{\partial x} - \left< p \right> \right) \psi(x) = 0 \]
Letting $y = x - \left< x \right>$ and $p_0 = \left< p \right>$ then, 
\[ \frac{\partial}{\partial y} \psi(y) = \left( \frac{y}{\hbar \alpha} + i \frac{p_0}{\hbar} \right) \psi(y)\text{ so } \psi(x) = N \exp{\left[ \frac{y^2}{2 \hbar \alpha} + i \frac{p_0}{\hbar} y \right]}  = N \exp{\left[ - \frac{y^2}{4 \Delta x^2} + i \frac{p_0}{\hbar} y \right]} \]
Thus, \[\psi(x) = \frac{1}{(2 \pi)^\frac{1}{4} (\Delta x)^\frac{1}{2}} \exp{\left[ -\frac{(x - x_0)^2}{4 \Delta x^2} + i \frac{p_0}{\hbar} (x - x_0) \right]}\]


\section*{Problem 11.}

Consider $F(\alpha) = e^{\alpha A} e^{\alpha B}$ then 
\[\deriv{}{\alpha} F(\alpha) = A e^{\alpha A} e^{\alpha B} +  e^{\alpha A} B e^{\alpha B} = A e^{\alpha A} e^{\alpha B} +  e^{\alpha A} B e^{-\alpha A}  e^{\alpha A} e^{\alpha B} = (A + e^{\alpha A} B e^{-\alpha A})F(\alpha)\]
However, \[\deriv{}{\alpha} e^{\alpha A} B e^{-\alpha A} = e^{\alpha A} A B e^{-\alpha A} - e^{\alpha A} BA e^{-\alpha A} = e^{\alpha A} [A, B] e^{-\alpha A}\]
Now since $[A, B]$ commutes with both $A$ and $B$ we have,
\[ \deriv{}{\alpha} e^{\alpha A} B e^{-\alpha A} = [A, B] e^{\alpha A} e^{-\alpha A} = [A, B]\]
Therefore, because $[A, B]$ is independent of $\alpha$,
\[e^{\alpha A} B e^{-\alpha A} =  e^{\alpha A} B e^{-\alpha A} \big|_{\alpha = 0}   + \alpha [A, B] = B + \alpha [A, B] \]
Applying this result above, 
\[ \deriv{}{\alpha} F(\alpha) = (A + B + \alpha [A, B])F(\alpha) \]
Thus,
\[ F(\alpha) = F(0) e^{\alpha A + \alpha B + \frac{\alpha^2}{2} [A, B]} = e^{\alpha A + \alpha B + \frac{\alpha^2}{2} [A, B]}\]

Evaluating at $\alpha = 1$, 
\[F(1) = e^A e^B = e^{A + B + \frac{1}{2} [A, B]}\]

\end{document}

