\documentclass[12pt]{extarticle}
\include{QuantumCommands}

\begin{document}
\atitle{5}
 
\section*{Problem 16.}

\begin{enumerate}
\item Let $\hat{B}(\Delta p) = e^{i \Delta p \hat{x} /\hbar}$ then consider \[\deriv{}{p_0} \hat{B}^\dagger(p_0) \hat{p} \hat{B}(p_0) =  \frac{i}{\hbar} \hat{B}^\dagger(p_0) \hat{p}  \hat{x} \hat{B}(p_0) \hat{p} -  \frac{i}{\hbar} \hat{B}^\dagger(p_0) \hat{x} \hat{p} \hat{B}(p_0)  =  \frac{-i}{\hbar} \hat{B}^\dagger(p_0)[\hat{x}, \hat{p}] \hat{B}(p_0) = 1 \]
Thus, \[ \hat{B}^\dagger(p_0) \hat{p} \hat{B}(p_0) = \hat{B}^\dagger(0) \hat{p} \hat{B}(0) + p_0 = \hat{p} + p_0\]
Therefore, applying the operator, $\ket{\psi_{\Delta p}} = \hat{B}(\Delta p) \ket{\psi}$
then \[\bra{\psi_{\Delta p}} \hat{p} \ket{\psi_{\Delta p}} = \bra{\psi} \hat{B}^\dagger(\Delta p) \hat{p} \hat{B}(\Delta p) \ket{\psi} = \bra{\psi} (\hat{p} + \Delta p)\ket{\psi} = \left< \hat{p} \right> + \Delta p\]

\item We can write $\hat{x} = \sqrt{\frac{\hbar}{2 m \omega}} (\adag + \a)$ so letting $\alpha = \sqrt{\frac{\hbar}{2 m \omega}} \frac{\Delta p}{\hbar}$ we have, \[ \hat{B}(\Delta p) = e^{i \alpha (\adag + \a)}\]
then because $[\a, \adag] = 1$ which commutes with everything, so we can apply \[e^{\hat{A} + \hat{B}}  = e^{\hat{A}} e^{\hat{B}} e^{-\frac{1}{2} [\hat{A}, \hat{B}]}\]
Thus, 
\[ \hat{B}(\Delta p) = e^{i \alpha \adag} e^{i \alpha \a} e^{- \frac{1}{2} \alpha^2 (\Delta p)^2}\]
However, \[e^{i \alpha \a } \ket{0} = \left(1 + i \alpha \a + \frac{1}{2} (i \alpha \a)^2 + \cdots \right) \ket{0} = \ket{0}\]
and therefore, \[ \ket{\psi} = \hat{B}(\Delta p) \ket{0} = e^{-\frac{1}{2} \alpha^2 (\Delta p)^2} e^{i  \alpha \adag} \ket{0}\]
Expanding the exponential, 
\[ \ket{\psi} = e^{-\frac{1}{2} \alpha^2 (\Delta p)^2} \sum_{n = 0}^{\infty} \frac{(i \alpha \Delta p)^n}{n!} (\adag)^n \ket{0} = e^{-\frac{1}{2} \alpha^2} \sum_{n = 0}^{\infty} \frac{(i \alpha)^n}{\sqrt{n!}} \ket{n} \]
Therefore, we can read off the propabilities,
\[P(0) = | \inner{0}{\psi} |^2 = e^{-\alpha^2}  = \exp{\left[-\frac{(\Delta p)^2 }{2 m \omega \hbar} \right]}\]
\item Simiarly, 
\[P(n) = | \inner{n}{\psi} |^2 = \frac{\alpha^{2n} e^{-\alpha^2}}{n!} = \frac{1}{n!} \left(\frac{(\Delta p)^2}{2 m \omega \hbar} \right)^n \exp{\left[-\frac{(\Delta p)^2 }{2 m \omega \hbar} \right]} \]
\end{enumerate}

\section*{Problem 17.}

\begin{enumerate}
\item Let \[\hamilt = \frac{1}{2m} \left(\hat{p}_x^2 + (\hat{p}_y - q A_y)^2 + \hat{p}_z^2 \right) = \frac{1}{2m} \left(\hat{p}_x^2 + (\hat{p}_y - q B \hat{x})^2 + \hat{p}_z^2 \right) \]
Because $[\hamilt, \hat{p}_y] = 0$ and $[\hamilt, \hat{p}_z] = 0$ and $[\hat{p}_y, \hat{p}_z] = 0$ we can find simultaneous eigenstates of the three operators. We search for solutions of the form $\ket{\psi} = \ket{\psi_x} \otimes \ket{p_y} \otimes \ket{p_z}$ with $\hat{p}_y \ket{p_y} = p_y \ket{p_y}$ and $\hat{p}_z \ket{p_z} = p_z \ket{p_z}$. Then, using the commutation relations, \[ \hamilt \ket{\psi} = \frac{1}{2m} \left(\hat{p}_x^2 + (p_y - q B \hat{x})^2 + p_z^2 \right) \ket{\psi_x} \otimes \ket{p_y} \otimes \ket{p_z}  \]  
Then 
\[ \hamilt \ket{\psi} = \left[ \frac{1}{2m} \hat{p}_x^2 + \frac{1}{2} m \omega^2 \left(\hat{x} - \frac{p_y}{q B} \right)^2 + \frac{p_z^2}{2m} \right] \ket{\psi_x} \otimes \ket{p_y} \otimes \ket{p_z}  \] 
where $\omega = \frac{qB}{m}$. Then define the lowering operator,
\[\a_{p_y} = \sqrt{\frac{m \omega}{2 \hbar}} \left(\hat{x} - \frac{p_y}{q B} + i \frac{\hat{p}_x}{m \omega} \right) \]
as before, this operators satisfies the commutation relation $[\a_{p_y}, \adag_{p_y}] = 1$ and,
\[ \adag_{p_y} \a_{p_y} = \frac{1}{\hbar \omega} \left[ \frac{1}{2m} \hat{p}_x^2 + \frac{1}{2} m \omega^2 \left(\hat{x} - \frac{p_y}{q B} \right)^2 \right] - \frac{1}{2}\]   
Thus, 
\[ \hamilt \ket{\psi} = \left[ \hbar \omega \left(\adag_{p_y} \a_{p_y} + \frac{1}{2} \right) + \frac{p_z^2}{2m} \right] \ket{\psi_x} \otimes \ket{p_y} \otimes \ket{p_z}  \]
The eigenstates of $\adag_{p_y} \a_{p_y}$ are $\ket{\psi_x} = \ket{n}$ with $\adag_{p_y} \a_{p_y} \ket{n} = n \ket{n}$ Therefore the spectrum is given by, 
\[E_{n, p_z} = \hbar \omega \left(n + \frac{1}{2} \right) + \frac{p_z^2 }{2m}\]
which are independent of $p_y$. 

\item
Consider the states: $\a_{p_y} \ket{\alpha, p_y} = \alpha \ket{\alpha, p_y}$ in the $x$-momentum basis:
\[ \bra{p_x} \a_{p_y} \ket{\alpha, p_y} = \sqrt{\frac{m \omega}{2 \hbar}} \left( i \hbar \pderiv{}{p_x} - \frac{p_y}{q B} + \frac{i p_x}{m \omega} \right) \tilde{\psi}_\alpha(p_x) = \alpha \tilde{\psi}_\alpha(p_x)\]
where I have used the fact that, in the momentum basis,
\[\bra{p_x} \hat{x} \ket{\psi} = i \hbar \pderiv{}{p_x} \inner{p_x}{\psi} = i \hbar \pderiv{}{p_x} \tilde{\psi}(p_x)\]
Furthermore, we can write:
\begin{align*}
\hat{x} &= \sqrt{\frac{\hbar}{2m \omega}} \left(\a_{p_y} + \adag_{p_y} \right) + \frac{p_y}{q B}  \\ 
\hat{p} &= \frac{m \omega}{2i} \sqrt{\frac{2\hbar}{m \omega}} \left(\a_{p_y} - \adag_{p_y}\right)
\end{align*}
and thus,

\begin{align*}
\bra{\alpha, p_y} \hat{x} \ket{\alpha, p_y} &= \sqrt{\frac{2\hbar}{m \omega}} \: \mathfrak{Re}[\alpha] + \frac{p_y}{q B} = x_0(p_y) \\ 
\bra{\alpha, p_y} \hat{p}_x \ket{\alpha, p_y} &= \sqrt{{2 \hbar m \omega}} \: \mathfrak{Im}[\alpha] = p_{x,0}
\end{align*}
Therefore, I define the following quantities, $x_0$, $y_0$, $z_0$, $p_{x,0}$, $p_{y,0}$, and $p_{z,0}$ are the classical initial conditions about which the probability distributions will be peaked and the characteristic scalles: $x_c = \sqrt{\frac{\hbar}{m \omega}}$ and $p_c = \sqrt{\hbar m \omega}$. Now, let

\[\alpha = \frac{1}{\sqrt{2}} \left[ \frac{1}{x_c} \left(x_0 - \frac{p_{y,0}}{qB} \right) + i \frac{p_{x,0}}{p_c} \right] \]
so that the expectation values of the coherent state corresponding to the classical initial value of $p_y$ agree with the classical initial conditions. Now, we know that (see addendum)
\begin{align*} 
e^{-i \hamilt t/\hbar} \ket{\alpha} \otimes \ket{p_y} \otimes \ket{p_z} &= e^{-i \left(\frac{1}{2} \omega  + \frac{p_z^2}{2\hbar m} \right) t} e^{-i \adag_{p_y} \a_{p_y} t/ \hbar} \ket{\alpha} \otimes \ket{p_y} \otimes \ket{p_z} \\ 
& = e^{-i \left(\frac{1}{2} \omega  + \frac{p_z^2}{2\hbar m} \right) t} \ket{\alpha e^{-i \omega t}} \otimes \ket{p_y} \otimes \ket{p_z}
\end{align*}
Therefore, we can solve for the time dependent momentum space wavefunction representing the state $\ket{\alpha} \otimes \ket{p_y} \otimes \ket{p_z}$ as follows, 
\[ \left( i \hbar \pderiv{}{p_x} - \frac{p_y}{q B} + \frac{i p_x}{m \omega} - \sqrt{\frac{2 \hbar}{m \omega}} \alpha e^{-i \omega t} \right) \tilde{\psi}_\alpha(p_x, t) = 0\]
Expainding $\alpha$, 
\[ \left( \pderiv{}{p_x} + i \frac{p_y}{q B \hbar} + \frac{p_x}{\hbar m \omega} + i \left[\frac{1}{\hbar} \left(x_0 - \frac{p_{y,0}}{q B} \right) + i \frac{p_{x,0}}{\hbar m \omega} \right] e^{-i \omega t} \right) \tilde{\psi}_\alpha(p_x, t) = 0 \]
Let $g_0 = \left(x_0 - \frac{p_{y,0}}{q B} \right)$
\begin{align*}
\pderiv{}{p_x} \tilde{\psi}_\alpha(p_x, t) = - \left( i \frac{p_y}{q B \hbar} + \frac{p_x}{p_c^2} + i \frac{g_0}{\hbar} \cos{\omega t} + \frac{g_0}{\hbar} \sin{\omega t} - \frac{p_{x,0}}{p_c^2} \cos{\omega t} + i \frac{p_{x,0}}{p_c^2} \sin{\omega t} \right)\tilde{\psi}_\alpha(p_x, t)
\end{align*}
Therefore, 
\begin{align*}
\tilde{\psi}_\alpha(p_x, t) = N(t) & \exp{\left[-\frac{i}{\hbar} \left(\frac{p_y}{qB} + g_0 \cos{\omega t} + \frac{p_{x, 0}}{m \omega} \sin{\omega t} \right) (p_x - p_{x,0}) \right]} \\ \cdot & \exp{\left[ -\frac{1}{2 p_c^2} \Big( p_x - p_{x,0} \cos{\omega t} + g_0 m \omega \sin{\omega t} \Big)^2 \right]}
\end{align*}
\end{enumerate}
Where we have choosen the phase to be zero at the initial momentum as to not bias the initial positions. The first term is a pure momentum dependent phase and the second is a gaussian with $\sigma^2 = \frac{1}{2} p_c^2$ so matching the overall time dependent phase, 
\[N(t) = \frac{e^{-i \left(\frac{1}{2} \omega  + \frac{p_z^2}{2\hbar m} \right) t}}{\left(\pi p_c^2 \right)^{\frac{1}{4}}}\]  
Now, the Fourier transform of a definite momentum state is a delta function in $p$-space so the full wavefunction in momentum space is:
\begin{align*}
\tilde{\psi}_{\bar{p}_y, \bar{p}_z} (p_x, p_y, p_z, t) = \frac{1}{\left(\pi p_c^2 \right)^{\frac{1}{4}}} & \exp{\left[-\frac{i}{\hbar} \left(\frac{p_y}{qB} + g_0 \cos{\omega t} + \frac{p_{x, 0}}{m \omega} \sin{\omega t} \right) (p_x - p_{x,0}) \right]} \\ \cdot & \exp{\left[ -\frac{i}{\hbar} \left(\frac{1}{2} \hbar \omega  + \frac{p_z^2}{2 m} \right) t \right]} \exp{\left[ -\frac{1}{2 p_c^2} \Big( p_x - p_{x,0} \cos{\omega t} + g_0 m \omega \sin{\omega t} \Big)^2 \right]} \\ \cdot \: & \delta(p_y - \bar{p}_y) \delta(p_z - \bar{p}_z)
\end{align*}  
Now, we construct a wavepacket by superimposing these wavefunctions with coeficients peaked about $\bar{p}_x = p_{x,0}$ and $\bar{p}_y = p_{y, 0}$ and with phases $e^{-i \bar{p}_y y_0 /\hbar}$ and $e^{-i \bar{p}_z z_0 /\hbar}$ to shift the distribution to the initial positions. Thus,
\begin{align*}
\tilde{\psi} (p_x, p_y, p_z, t) & = \int \tilde{\psi}_\alpha(p_x, t) \delta(p_y - \bar{p}_y) \delta(p_z - \bar{p}_z) C(\bar{p}_y, \bar{p}_z) e^{-i \bar{p}_y y_0 /\hbar} e^{-i \bar{p}_z z_0 /\hbar} \: \d{\bar{p}_y} \d{\bar{p}_z} \\
 & = \psi_\alpha(p_x, t)  C(p_y, p_z) e^{-i p_y y_0 /\hbar} e^{-i p_z z_0 /\hbar}
\end{align*} 
Therefore, in all its horrifying glory,
\begin{align*}
\tilde{\psi} (p_x, p_y, p_z, t) = \frac{1}{\left(\pi p_c^2 \right)^{\frac{1}{4}}} & \exp{\left[-\frac{i}{\hbar} \left(\frac{p_y}{qB} + g_0 \cos{\omega t} + \frac{p_{x, 0}}{m \omega} \sin{\omega t} \right) (p_x - p_{x,0}) \right]} \\ \cdot & \exp{\left[ -\frac{i}{\hbar} \left(\frac{1}{2} \hbar \omega  + \frac{p_z^2}{2 m} \right) t \right]} \exp{\left[ -\frac{1}{2 p_c^2} \Big( p_x - p_{x,0} \cos{\omega t} + g_0 m \omega \sin{\omega t} \Big)^2 \right]} \\ \cdot & \:  C(p_y, p_z) e^{-i p_y y_0 /\hbar} e^{-i p_z z_0 /\hbar}
\end{align*} 
Finally, we apply the inverse Fourier transform, 
\begin{align*}
\psi & (x, y, z, t) =  \\  & \int \frac{1}{\left(\pi p_c^2 \right)^{\frac{1}{4}}\sqrt{2 \pi \hbar}} \exp{\left[-\frac{i}{\hbar} \left(\frac{p_y}{qB} + g_0 \cos{\omega t} + \frac{p_{x, 0}}{m \omega} \sin{\omega t} \right) (p_x - p_{x,0})  \right]} \exp{\left[ -\frac{i}{\hbar} \left(\frac{1}{2} \hbar \omega  + \frac{p_z^2}{2 m} \right) t \right]} \\ & \quad \cdot \exp{\left[ -\frac{1}{2 p_c^2} \Big( p_x - p_{x,0} \cos{\omega t} + g_0 m \omega \sin{\omega t} \Big)^2 \right]}  C(p_y, p_z) e^{-i p_y y_0 /\hbar} e^{-i p_z z_0 /\hbar} e^{i (p_x x + p_y y + p_z z)/\hbar} \mathrm{d}^3 p
\end{align*} 
and collct the totall phase,
\[\Phi = p_x x + p_y (y-y_0) + p_z (z - z_0) - \left(\frac{1}{2} \hbar \omega + \frac{p_z^2}{2m} \right) t - \left( \frac{p_y}{qB} + g_0 \cos{\omega t} + \frac{p_{x, 0}}{m \omega} \sin{\omega t} \right) (p_x - p_{x,0})\] 
so the integral can be written as,
\begin{align*}
\psi (x, y, z, t) = \frac{1}{\left(\pi p_c^2 \right)^{\frac{1}{4}}\sqrt{2 \pi \hbar}} \int  e^{i \Phi / \hbar} \exp{\left[ -\frac{1}{2 p_c^2} \Big( p_x - p_{x,0} \cos{\omega t} + g_0 m \omega \sin{\omega t} \Big)^2 \right]}  C(p_y, p_z)  \mathrm{d}^3 p
\end{align*} 
which is maximized at points where the phase is stationary at the peak values of the weigting coeficients. That is, the wavefunction is maximized at points where,
\[\nabla_{\vec{p}} \: \Phi \Big|_{\vec{p}_m(t)} = 0\]
Thus, 
\begin{align*}
\pderiv{\Phi}{p_x} & = x - \left( \frac{p_{y,0}}{qB} + \left(x_0 - \frac{p_{y,0}}{q B} \right) \cos{\omega t} + \frac{p_{x, 0}}{m \omega} \sin{\omega t} \right) = 0 \\
\pderiv{\Phi}{p_y} & = y - y_0 - \frac{p_{x,m}(t) - p_{x,0}}{q B} = 0 \\
\pderiv{\Phi}{p_z} & = z - z_0 - \frac{p_{z,0}}{m} t = 0
\end{align*}
Where $p_{x,m}(t)$ maximizes the gaussian, i.e. $p_{x,m}(t) = p_{x, 0} \cos{\omega t} - \left(x_0 - \frac{p_{y,0}}{q B} \right) m \omega \sin{\omega t}$ \\
Therefore, the maximum of the wavefunction evolves as:
\begin{align*}
x & =  \frac{p_{y,0}}{qB} + \left(x_0 - \frac{p_{y,0}}{q B} \right) \cos{\omega t} + \frac{p_{x, 0}}{m \omega} \sin{\omega t} \\
y & = y_0 - \frac{p_{x, 0}}{qB}(1 - \cos{\omega t}) - \left(x_0 - \frac{p_{y,0}}{q B} \right) \frac{m \omega}{qB} \sin{\omega t} \\
z & = z_0 + \frac{p_{z,0}}{m} t
\end{align*}
Notice that $\frac{m \omega}{qB} = 1$ because $\omega = \frac{qB}{m}$ by definition. Also, if we make the identifications, 
\begin{align*}
v_{x,0} & = \frac{p_{x,0}}{m} \\
v_{y,0} & = \frac{p_{y,0} - qB x_0}{m} \\
v_{z,0} & = \frac{p_{z,0}}{m}
\end{align*}
then we have,
\begin{align*}
x & =  \frac{m}{qB} v_{y,0} + x_0 - \frac{m}{qB} v_{y,0} \cos{\omega t} + \frac{v_{x, 0}}{ \omega} \sin{\omega t} \\
y & = y_0 - \frac{m}{qB} v_{x, 0}(1 - \cos{\omega t}) + \frac{m}{qB} v_{y,0} \sin{\omega t} \\
z & = z_0 + v_{z,0} t
\end{align*}
and therefore, simplifying, 
\begin{align*}
x & =  x_0  + \frac{v_{y,0}}{\omega}(1 - \cos{\omega t}) + \frac{v_{x, 0}}{ \omega} \sin{\omega t} \\
y & = y_0 - \frac{v_{x, 0}}{\omega} (1 - \cos{\omega t}) + \frac{v_{y,0}}{\omega} \sin{\omega t} \\
z & = z_0 + v_{z,0} t
\end{align*}
which is exactly a clockwise (from above) circular helix, the motion of a classical charged particle in a constant magnetic field. The frequency of the circular orbit is \[\omega = \frac{qB}{m}\]
which is the Larmor precession frequency. 

\section*{Problem 18.}

\begin{enumerate}
\item Define $e^{- i \hat{\phi}} = \frac{1}{\sqrt{1 + \adag \a}} \a$ then \[e^{- i \hat{\phi}} \ket{n} = \frac{1}{\sqrt{1 + \adag \a}} \sqrt{n} \ket{n-1}\]
but $\ket{n-1}$ is an eigenstate of $\adag \a$ so \[e^{- i \hat{\phi}} \ket{n} = \sqrt{n} \frac{1}{\sqrt{1 + (n - 1)}} \ket{n-1} = \ket{n-1}\]

\item $e^{i \hat{\phi}} = \left(e^{- i \hat{\phi}}\right)^\dagger = \adag \frac{1}{\sqrt{1 + \adag \a}}$ because $\adag \a$ is Hermitian. Then, \[e^{i \hat{\phi}} \ket{n} = \adag \frac{1}{\sqrt{1 + \adag \a}} \ket{n} = \adag \frac{1}{\sqrt{1 + n}} \ket{n} = \ket{n+1}\]

\item Since $\frac{1}{\sqrt{1 + \adag \a}}$ is a function of $\adag \a$ alone, it commutes with $\adag \a$. Thus, 
\begin{align*}
[\adag \a, e^{- \hat{\phi}}] &= \adag \a \frac{1}{1 + \adag \a} \a - \frac{1}{1 + \adag \a} \a \adag \a = \frac{1}{1 + \adag \a} \adag \a \a - \frac{1}{1 + \adag \a} (\adag \a + [\a, \adag]) \a \\ & = - \frac{1}{1 + \adag \a} [\a, \adag] = - \frac{1}{1 + \adag \a} = - e^{- i \hat{\phi}} 
\end{align*}

\item Define: \[\sin{\hat{\phi}} = \frac{1}{2i} \left( e^{i \hat{\phi}} - e^{-i \hat{\phi}} \right)\] and let, \[\ket{\phi_0} = \sum_{n = 0}^{\infty} c_n (\phi_0) \ket{n}\]
such that, 
\begin{align*}
\sin{\hat{\phi}} \ket{\phi_0} &= \frac{1}{2i} \sum_{n = 0}^{\infty} \left( e^{i \hat{\phi}} - e^{-i \hat{\phi}} \right) c_n (\phi_0) \ket{n}  = \sin{\phi_0} \ket{\phi_0} \\ 
\sin{\hat{\phi}} \ket{\phi_0} &= \frac{1}{2i} \sum_{n = 0}^{\infty} \left( \ket{n + 1} - \ket{n - 1} \right) c_n (\phi_0) = \sin{\phi_0} \sum_{n = 0}^{\infty} c_n (\phi_0) \ket{n} \\ 
& = \frac{1}{2i} \left( \sum_{n = 1}^{\infty} c_{n - 1} (\phi_0) \ket{n}   - \sum_{n = 0}^{\infty} c_{n + 1} (\phi_0) \ket{n} \right)\\ & = \frac{1}{2i}  \sum_{n = 1}^{\infty} (c_{n - 1}(\phi_0) - c_{n + 1} (\phi_0)) \ket{n} - \frac{1}{2i} c_1(\phi_0) \ket{0}
\end{align*}
matching terms,
\[ -\frac{1}{2i} c_1(\phi_0) = c_0(\phi_0) \sin{\phi_0}\]
and 
\[c_{n + 1} (\phi_0) = c_{n - 1}(\phi_0) - (2i \sin{\phi_0}) c_{n}(\phi_0) \]
this recurrence relation can be easily solved by finding characteristic roots or using generating functions. I will not waste your time with that here; I will simply write out the solution.
\[c_n = N(\phi_0) \left[(-1)^n e^{i \phi_0 (n + 1)} + e^{- i \phi_0 (n + 1)} \right]\]
And thus, writting the series explicitly,
\[\ket{\phi_0} = N(\phi_0) \sum_{n = 0}^\infty \left[(-1)^n e^{i \phi_0 (n + 1)} + e^{- i \phi_0 (n + 1)} \right] \ket{n} \]

\item In an exactly analogous manner, define: \[\cos{\hat{\phi}} = \frac{1}{2} \left( e^{i \hat{\phi}} + e^{-i \hat{\phi}} \right)\] and let, \[\ket{\phi_0} = \sum_{n = 0}^{\infty} c_n (\phi_0) \ket{n}\]
such that, 
\begin{align*}
\cos{\hat{\phi}} \ket{\phi_0} &= \frac{1}{2} \sum_{n = 0}^{\infty} \left( e^{i \hat{\phi}} + e^{-i \hat{\phi}} \right) c_n (\phi_0) \ket{n}  = \cos{\phi_0} \ket{\phi_0} \\ 
\cos{\hat{\phi}} \ket{\phi_0} &= \frac{1}{2} \sum_{n = 0}^{\infty} \left( \ket{n + 1} + \ket{n - 1} \right) c_n (\phi_0) = \cos{\phi_0} \sum_{n = 0}^{\infty} c_n (\phi_0) \ket{n} \\ 
& = \frac{1}{2} \left( \sum_{n = 1}^{\infty} c_{n - 1} (\phi_0) \ket{n}  + \sum_{n = 0}^{\infty} c_{n + 1} (\phi_0) \ket{n} \right)\\ & = \frac{1}{2}  \sum_{n = 1}^{\infty} (c_{n - 1}(\phi_0) + c_{n + 1} (\phi_0)) \ket{n} + \frac{1}{2} c_1(\phi_0) \ket{0}
\end{align*}
matching terms,
\[ \frac{1}{2} c_1(\phi_0) = c_0(\phi_0) \cos{\phi_0}\]
and 
\[c_{n + 1} (\phi_0) = (2 \cos{\phi_0}) c_{n}(\phi_0) - c_{n - 1}(\phi_0) \]
this recurrence relation can be easily solved by finding characteristic roots or using generating functions. I will not waste your time with that here; I will simply write out the solution.
\[c_n = N(\phi_0) \left[e^{i \phi_0 (n + 1)} - e^{- i \phi_0 (n + 1)} \right]\] 
And thus, writting the series explicitly,
\[\ket{\phi_0} = N(\phi_0) \sum_{n = 0}^\infty \left[e^{i \phi_0 (n + 1)} + e^{- i \phi_0 (n + 1)} \right] \ket{n} \]  
\end{enumerate}

\section*{Addendum}
We want to show that for $\hamilt = \hbar \omega \left(\adag \a + \frac{1}{2}\right)$ the time evolution operator acts as, \[e^{-i\hamilt t/\hbar} \ket{\alpha} = e^{-\frac{1}{2} i \omega t} \ket{\alpha e^{-i \omega t}}\]
In the energy basis, 
\[\ket{\alpha} = \sum_{n = 0}^\infty \frac{\alpha^n}{\sqrt{n!}} \ket{n}\]
but each eigenstate evolves nicely,
\[e^{- i \hamilt t / \hbar} \ket{n} = e^{- i \omega \adag \a t} e^{- \frac{1}{2} i \omega t} \ket{n} = e^{- i \omega n t} e^{- \frac{1}{2} i \omega t} \ket{n}\]
Therefore, 
\begin{align*}
e^{- i \hamilt t / \hbar} \ket{\alpha} & = e^{- \frac{1}{2} i \omega t} \sum_{n = 0}^\infty \frac{\alpha^n}{\sqrt{n!}} \: e^{- i \omega \adag \a t} \ket{n} = e^{- \frac{1}{2} i \omega t} \sum_{n = 0}^\infty \frac{\alpha^n e^{- i \omega n t} }{\sqrt{n!}} \ket{n} \\ & = e^{- \frac{1}{2} i \omega t} \sum_{n = 0}^\infty \frac{(\alpha e^{- i \omega t})^n }{\sqrt{n!}} \ket{n} = e^{-\frac{1}{2} i \omega t} \ket{\alpha e^{-i \omega t}}
\end{align*} 

\end{document}

